started working on semantics

src/fol/language.lean
@@ -12,29 +12,29 @@ noncomputable theory
 
 -- Sadly, lean does not support good inductive types.
 -- Hence we won't have arbitrary arity functions and relations.
-structure signature : Type :=
+structure Signature : Type :=
 (consts : ℕ)
 (funcs : ℕ)
 (ops : ℕ)
 (rels : ℕ)
 
 @[derive [decidable_eq]]
-structure Const (S : signature) : Type :=
+structure Const (S : Signature) : Type :=
 (const : ℕ)
 (const_le : const < S.consts)
 
 @[derive [decidable_eq]]
-structure Func (S : signature) : Type := 
+structure Func (S : Signature) : Type := 
 (func : ℕ)
 (func_le : func < S.funcs)
 
 @[derive [decidable_eq]]
-structure Op (S : signature) : Type := 
+structure Op (S : Signature) : Type := 
 (op : ℕ)
 (op_le : op < S.ops)
 
 @[derive [decidable_eq]]
-structure Rel (S : signature) : Type := 
+structure Rel (S : Signature) : Type := 
 (rel : ℕ)
 (rel_le : rel < S.rels)
 
@@ -42,16 +42,28 @@ structure Rel (S : signature) : Type :=
 def var := ℕ
 
 @[derive [decidable_eq]]
-inductive Term (S : signature) : Type
+inductive Term (S : Signature) : Type
 | Var : var → Term
 | ConstT : Const S → Term
 | FuncT : Func S → Term → Term   
 | OpT : Op S → Term → Term → Term
 
-instance {S : signature} : inhabited (Term S) :=
+instance var_has_coe {S : Signature} : has_coe var (Term S) :=
+⟨λ v, Term.Var v⟩
+
+instance const_has_coe {S : Signature} : has_coe (Const S) (Term S) :=
+⟨λ c, Term.ConstT c⟩
+
+instance func_has_coe {S : Signature} : has_coe_to_fun (Func S) (λ _, Term S → Term S) :=
+⟨λ f, Term.FuncT f⟩
+
+instance op_has_coe {S : Signature} : has_coe_to_fun (Op S) (λ _, Term S → Term S → Term S) :=
+⟨λ o, Term.OpT o⟩
+
+instance {S : Signature} : inhabited (Term S) :=
 ⟨Term.Var 0⟩
 
-def vars (S : signature) : Term S → set var := 
+def vars (S : Signature) : Term S → set var := 
 λ t, begin
   induction t with v c f t st o t₁ t₂ st₁ st₂,
   exact {v},
@@ -69,17 +81,17 @@ inductive Quantifier : Type
 | All : Quantifier
 
 @[derive [decidable_eq]]
-inductive Formula (S : signature) : Type
+inductive Formula (S : Signature) : Type
 | Eq : Term S → Term S → Formula
 | RelF : Rel S → Term S → Term S → Formula
 | Not : Formula → Formula
 | OpL  : LogicalOp → Formula → Formula → Formula
 | QuantifierL : Quantifier → var → Formula → Formula 
 
-instance {S : signature} : inhabited (Formula S) :=
+instance {S : Signature} : inhabited (Formula S) :=
 ⟨Formula.Eq (Term.Var 0) (Term.Var 0)⟩
 
-def free (S : signature) : Formula S → set var :=
+def free (S : Signature) : Formula S → set var :=
 λ φ, 
 begin
   induction φ with t₁ t₂ r t₁ t₂ φ sφ o φ₁ φ₂ sφ₁ sφ₂ q v φ sφ,
@@ -90,11 +102,11 @@ begin
   exact sφ \ {v},
 end
 
-def sentence {S : signature} (φ : Formula S) : Prop := free S φ = ∅ 
+def sentence {S : Signature} (φ : Formula S) : Prop := free S φ = ∅ 
 
 namespace language
 
-variable {S : signature}
+variable {S : Signature}
 
 section term
 
@@ -139,4 +151,4 @@ end free
 end language
 
 -- @[derive [has_mem, has_singleton Formula, has_union, has_emptyc, has_subset, complete_lattice]]
-def Theory (S : signature) := set (Formula S)
+def Theory (S : Signature) := set (Formula S)
