src/fol/semantics.lean
@@ -4,17 +4,73 @@ open language
 
 universe u
 
-structure Structure (S : signature) :=
-(Dom : Type u)
-(const : Const S → Dom)
-(func : Func S → Dom → Dom)
-(op : Op S → Dom → Dom → Dom)
-(rel : Rel S → Dom → Dom → Prop)
+structure Structure (S : Signature) :=
+(dom : Type u)
+(const : Const S → dom)
+(func : Func S → dom → dom)
+(op : Op S → dom → dom → dom)
+(rel : Rel S → dom → dom → Prop)
 
-variables {S : signature}
+instance {S : Signature} : has_coe_to_sort (Structure S) (Type u) := ⟨Structure.dom⟩
 
-def assignment (A : Structure S) := var → A.Dom
+variables {S : Signature}
 
-def subs_assignment {S : signature} {A : Structure S} 
-(β : assignment A) (a : A.Dom) (x : var) : assignment A :=
-λ v, ite (v = x) a (β v)
+structure assignment (A : Structure S) :=
+(ass : var → A)
+
+section assignment
+
+variable {A : Structure S}
+
+def subs_assignment (β : assignment A) (a : A) (x : var) : assignment A :=
+⟨λ v, ite (v = x) a (β.ass v)⟩ 
+
+notation _[_ / _] := subs_assignment
+
+def interp (β : assignment A) : Term S → A :=
+λ t,
+begin
+  induction t with v c f t a o t₁ t₂ a₁ a₂,
+  exact β.ass v,
+  exact A.const c,
+  exact A.func f a,
+  exact A.op o a₁ a₂
+end
+
+instance : has_coe_to_fun (assignment A) (λ _, Term S → A) :=
+⟨λ β, interp β⟩
+
+def eval : ∀ (β : assignment A) (φ : Formula S), Prop
+| β (Formula.Eq t₁ t₂) := β t₁ = β t₂ 
+| β (Formula.RelF R t₁ t₂) := A.rel R (β t₁) (β t₂)
+| β (Formula.Not φ) := ¬eval β φ
+| β (Formula.OpL LogicalOp.To φ₁ φ₂) := (eval β φ₁) → (eval β φ₂)
+| β (Formula.QuantifierL Quantifier.All v φ) := ∀ (a : A), eval (subs_assignment β a v) φ
+
+end assignment
+
+namespace semantics
+
+variable {A : Structure S}
+
+section interp
+
+lemma interp_var {β : assignment A} {v : var} : β v = β.ass v := rfl
+
+lemma interp_const {β : assignment A} {c : Const S} : β c = A.const c := rfl
+
+lemma interp_func {β : assignment A} {f : Func S} {t : Term S} : 
+interp β (f t) = A.func f (β t) := rfl
+
+lemma interp_op {β : assignment A} {o : Op S} {t₁ t₂ : Term S} :
+interp β (o t₁ t₂) = A.op o (β t₁) (β t₂) := rfl
+
+end interp
+
+section eval
+
+lemma eval_eq {β : assignment A} {t₁ t₂ : Term S} 
+
+end eval
+
+end semantics
